Prove the owner's rights in zcb

proofs/zero_coupon_bond.v
@@ -1,12 +1,546 @@
-Load helpers.
+Load metaproperties.
 
-Definition zero_coupon_bond
+(* Zero coupon bond *)
+Definition zcb_desc
            (NOW : nat)
            (PERIOD : nat) :=
   (And
      (Give (Scale 10 (One USD)))
      (At (NOW + PERIOD) (Scale 11 (One USD)))
   ).
+
+Lemma zcb_execute_O_to_I :
+  forall sc now period I O bal time gtw ctr_id dsc_id next_id ledger result,
+    execute (zcb_desc now period)  sc I O bal time gtw ctr_id dsc_id next_id ledger =
+    Some result ->
+    exists tr,
+      In tr (res_ledger result) /\
+      tr_ctr_id tr = ctr_id /\
+      tr_from tr = O /\
+      tr_to tr = I /\
+      tr_amount tr = sc * 10 /\
+      tr_timestamp tr = time.
+Proof.
+  unfold zcb_desc. intros.
+  simpl in H.
+  case_analysis H.
+  case_analysis H2; simpl in *.
+  - eexists.
+    split.
+    + right. left. trivial.
+    + repeat split; trivial.
+  - eexists.
+    split.
+    + left. trivial.
+    + repeat split; trivial.
+Qed.
+
+
+Lemma zcb_execute_I_to_O :
+  forall sc now period I O bal time gtw ctr_id dsc_id next_id ledger result,
+    execute (zcb_desc now period)  sc I O bal time gtw ctr_id dsc_id next_id ledger =
+    Some result ->
+    exists tr,
+      In tr (res_ledger result) /\
+      tr_ctr_id tr = ctr_id /\
+      tr_from tr = I /\
+      tr_to tr = O /\
+      tr_amount tr = sc * 11 /\
+      tr_timestamp tr = time.
+Proof.
+  unfold zcb_desc. intros.
+  simpl in H.
+  case_analysis H.
+  case_analysis H2; simpl in *.
+  - eexists.
+    split.
+    + left. trivial.
+    + repeat split; trivial.
+  - admit. (* This case cannot be proved. Timebounds generates a new contract.  *)
+Admitted.
+
+Lemma zcb_execute_I_to_O_new_ctr :
+  forall sc now period I O bal time gtw ctr_id dsc_id next_id ledger result,
+    execute (zcb_desc now period)  sc I O bal time gtw ctr_id dsc_id next_id ledger =
+    Some result ->
+    (exists tr,
+      In tr (res_ledger result) /\
+      tr_ctr_id tr = ctr_id /\
+      tr_from tr = I /\
+      tr_to tr = O /\
+      tr_amount tr = sc * 11 /\
+      tr_timestamp tr = time) \/
+    exists ctr,
+      In ctr (res_contracts result) /\
+      ctr_primitive ctr = (At (now + period) (Scale 11 (One USD))) /\
+      ctr_issuer ctr = I /\
+      ctr_owner ctr = O /\
+      ctr_scale ctr = sc.
+Proof.
+  unfold zcb_desc. intros.
+  simpl in H.
+  case_analysis H.
+  case_analysis H2; simpl in *.
+  - left. eexists.
+    split.
+    + left. trivial.
+    + repeat split; trivial.
+  - right.
+    eexists. split.
+    + left. trivial.
+    + simpl. unfold At. repeat split; trivial.
+Qed.
+
+
+Lemma zcb_step_O_to_I :
+  forall s1 s2 ctr_id dsc_id now period I O sc ctr,
+    step s1 s2 ->
+    consistent_state s1 ->
+    ctr = finctr ctr_id dsc_id (zcb_desc now period) I O O sc ->
+    In ctr (m_contracts s1) ->
+    ~ In (Executed ctr_id) (m_events s1) ->
+    In (Executed ctr_id) (m_events s2) ->
+    O <> 0 ->
+    exists tr,
+      In tr (m_ledger s2) /\
+      tr_ctr_id tr = ctr_id /\
+      tr_from tr = O /\
+      tr_to tr = I /\
+      tr_amount tr = sc * 10 /\
+      tr_timestamp tr = (m_global_time s1).
+Proof.
+  intros.
+  assert (S := H).
+  induction H.
+  - subst s2. simpl in *.
+    destruct H4 as [H4 | H4]; try inversion H4; try contradiction.
+  - apply step_executes_only_one_contract
+      with (ctr := ctr) (ctr' := ctr0) in S; subst ctr; auto.
+    + subst ctr0 s2. simpl in *.
+      destruct H4 as [H4 | H4]; try contradiction.
+      unfold exec_ctr_in_state_with_owner in H11.
+      apply zcb_execute_O_to_I in H11.
+      destruct H11 as [tr H11].
+      exists tr. simpl in H11.
+      unfold can_join in H6.
+      simpl in H6.
+      destruct H6 as [H6 | H6]; auto.
+      ++ subst owner. auto.
+      ++ contradiction.
+    + subst s2. simpl in *. left. trivial.
+  - apply step_executes_only_one_contract
+      with (ctr := ctr) (ctr' := ctr0) in S; subst ctr; auto.
+    + subst ctr0. simpl in *. unfold zcb_desc in H8. inversion H8.
+    + subst s2. simpl in *. left. trivial.
+  - apply step_executes_only_one_contract
+      with (ctr := ctr) (ctr' := ctr0) in S; subst ctr; auto.
+    + subst ctr0. simpl in *. unfold zcb_desc in H8. inversion H8.
+    + subst s2. simpl in *. left. trivial.
+  - apply step_executes_only_one_contract
+      with (ctr := ctr) (ctr' := ctr0) in S; subst ctr; auto;
+      subst s2; simpl in *;
+        destruct H4 as [H4 | H4]; try inversion H4; try contradiction.
+  - subst s2. simpl in *. contradiction.
+Qed.
+
+
+Lemma zcb_steps_O_to_I :
+  forall s1 s2 ctr_id dsc_id now period I O sc ctr,
+    steps s1 s2 ->
+    consistent_state s1 ->
+    ctr = finctr ctr_id dsc_id (zcb_desc now period) I O O sc ->
+    In ctr (m_contracts s1) ->
+    ~ In (Executed ctr_id) (m_events s1) ->
+    In (Executed ctr_id) (m_events s2) ->
+    O <> 0 ->
+    exists time tr,
+      In tr (m_ledger s2) /\
+      tr_ctr_id tr = ctr_id /\
+      tr_from tr = O /\
+      tr_to tr = I /\
+      tr_amount tr = sc * 10 /\
+      tr_timestamp tr = time.
+Proof.
+  intros.
+  induction H.
+  - subst. contradiction.
+  - assert (H' := H).
+    apply steps_preserves_consistent_state in H'; auto.
+    apply steps_effect_over_contract with (ctr := ctr) in H; trivial.
+    destruct H as [H|[H|H]]; trivial.
+    + eexists.
+      eapply zcb_step_O_to_I; eauto.
+      destruct H' as [_ [_ [_ [T _]]]].
+      apply T in H.
+      destruct H as [H _]; subst ctr; auto.
+    + subst ctr. simpl in *.
+      apply IHsteps in H.
+      destruct H as [time [tr [H HT]]].
+      exists time, tr.
+      split; trivial.
+      eapply step_does_not_remove_transactions; eauto.
+    + eapply step_preserves_consistent_state in H'; eauto.
+      eapply step_does_not_remove_events in H6; eauto.
+      destruct H' as [_ [_ [_ [_ T]]]].
+      unfold not in T.
+      exfalso.
+      eapply T. subst ctr.
+      split; eauto.
+Qed.
+
+
+Lemma ltb_n_Sn:
+  forall n, n <? S n = true.
+Proof.
+  induction n; simpl; unfold Nat.ltb; trivial.
+Qed.
+
+
+Lemma leb_sound_true:
+  forall n m,
+    n <=? m = true -> n <= m.
+Proof.
+  induction n.
+  - induction m; intros; try omega.
+  - intros m.
+    case_eq m; intros; subst m; simpl in H0.
+    + inversion H0.
+    + apply IHn in H0. omega.
+Qed.
+
+
+Lemma leb_sound_false:
+  forall n m,
+    n <=? m = false -> ~ n <= m.
+Proof.
+  induction n.
+  - induction m; intros; simpl in H; inversion H.
+  - intros m.
+    case_eq m; intros; subst m; simpl in H0.
+    + omega.
+    + apply IHn in H0. omega.
+Qed.
+
+
+Lemma ltb_sound_true:
+  forall n m,
+    n <? m = true -> n < m.
+Proof.
+  unfold Nat.ltb.
+  intros.
+  simpl in H.
+  case_eq m; intros; subst m.
+  - inversion H.
+  - apply leb_sound_true in H. omega.
+Qed.
+
+
+Lemma ltb_sound_false:
+  forall n m,
+    n <? m = false -> ~ n < m.
+Proof.
+  unfold Nat.ltb.
+  intros.
+  simpl in H.
+  case_eq m; intros; subst m.
+  - omega.
+  - apply leb_sound_false in H. omega.
+Qed.
+
+
+SearchPattern (_ - _ < _).
+
+
+Lemma zcb_step_I_to_O :
+  forall s s' ctr_id dsc_id now period I O sc ctr,
+    step s s' ->
+    consistent_state s ->
+    ctr = finctr ctr_id dsc_id (zcb_desc now period) I O O sc ->
+    In ctr (m_contracts s) ->
+    ~ In (Executed ctr_id) (m_events s) ->
+    In (Executed ctr_id) (m_events s') ->
+    O <> 0 ->
+    m_global_time s = now + period ->
+    m_global_time s' = now + period ->
+    Δ <= now + period ->
+    exists time tr,
+      In tr (m_ledger s') /\
+      tr_ctr_id tr = ctr_id /\
+      tr_from tr = I /\
+      tr_to tr = O /\
+      tr_amount tr = sc * 11 /\
+      tr_timestamp tr = time.
+Proof.
+  intros.
+  induction H; subst s'; simpl in *.
+  - destruct H4 as [H4 | H4]; try inversion H4; try contradiction.
+  - destruct H4 as [H4 | H4].
+    case_eq (ctr_eq_dec ctr ctr0); intros; try contradiction.
+    + subst ctr0.
+      unfold can_join in H9.
+      destruct H9 as [H9 | H9]; intros.
+      * subst. simpl in *.
+        unfold exec_ctr_in_state_with_owner, zcb_desc in *.
+        simpl in *.
+        case_analysis H14.
+        case_analysis H16.
+        ** eexists. eexists.
+           split. simpl. left. trivial.
+           repeat split; trivial.
+        ** rewrite H7 in *.
+           apply ltb_sound_false in H9.
+           exfalso. unfold not in H9.
+           apply H9.
+           apply Nat.sub_lt; trivial.
+           unfold Δ. omega.
+      * subst ctr. simpl in *. subst. contradiction.
+    + contradiction.
+  - case_eq (ctr_eq_dec ctr ctr0); intros; try contradiction.
+    subst ctr0 ctr. unfold zcb_desc, ctr_primitive in *. inversion H11.
+  - case_eq (ctr_eq_dec ctr ctr0); intros; try contradiction.
+    subst ctr0 ctr. unfold zcb_desc, ctr_primitive in *. inversion H11.
+  - destruct H4 as [H4 | H4]; try inversion H4; try contradiction.
+  - contradiction.
+Qed.
+
+
+Lemma zcb_step_I_to_O_new_ctr :
+  forall s1 s2 ctr_id dsc_id now period I O sc ctr,
+    step s1 s2 ->
+    consistent_state s1 ->
+    ctr = finctr ctr_id dsc_id (zcb_desc now period) I O O sc ->
+    In ctr (m_contracts s1) ->
+    ~ In (Executed ctr_id) (m_events s1) ->
+    In (Executed ctr_id) (m_events s2) ->
+    O <> 0 ->
+    (exists time tr,
+      In tr (m_ledger s2) /\
+      tr_ctr_id tr = ctr_id /\
+      tr_from tr = I /\
+      tr_to tr = O /\
+      tr_amount tr = sc * 11 /\
+      tr_timestamp tr = time) \/
+    exists ctr,
+      In ctr (m_contracts s2) /\
+      ctr_primitive ctr = (At (now + period) (Scale 11 (One USD))) /\
+      ctr_issuer ctr = I /\
+      ctr_owner ctr = O /\
+      ctr_scale ctr = sc.
+Proof.
+  intros.
+  induction H; subst s2.
+  - simpl in *. destruct H4 as [H4 | H4]; try inversion H4.
+    contradiction.
+  - simpl in *. unfold exec_ctr_in_state_with_owner in H11.
+    unfold can_join in H6.
+    destruct H6 as [H6 | H6]; intros.
+    case_eq (ctr_eq_dec ctr ctr0); intros; try contradiction.
+    subst ctr0 ctr.
+    apply zcb_execute_I_to_O_new_ctr in H11.
+    simpl in *.
+    destruct H11 as
+        [[tr (A1 & A2 & A3 & A4 & A5 & A6)] |
+         [ctr (A1 & A2 & A3 & A4 & A5 )]].
+    + subst. left. exists (m_global_time s1), tr.
+      repeat split; trivial.
+    + subst. right. exists ctr.
+      repeat split; trivial.
+      apply in_app_iff. right. trivial.
+    + case_eq (ctr_eq_dec ctr ctr0); intros; try contradiction.
+      subst ctr0 ctr.
+      simpl in H6. subst O. contradiction.
+  - case_eq (ctr_eq_dec ctr ctr0); intros; try contradiction.
+    subst ctr0 ctr. unfold zcb_desc in *. simpl in *. inversion H8.
+  - case_eq (ctr_eq_dec ctr ctr0); intros; try contradiction.
+    subst ctr0 ctr. unfold zcb_desc in *. simpl in *. inversion H8.
+  - simpl in *. destruct H4 as [H4 | H4]. inversion H4. contradiction.
+  - simpl in *. contradiction.
+Qed.
+
+
+Lemma zcb_steps_I_to_O_new_ctr :
+  forall s1 s2 ctr_id dsc_id now period I O sc ctr,
+    steps s1 s2 ->
+    consistent_state s1 ->
+    ctr = finctr ctr_id dsc_id (zcb_desc now period) I O O sc ->
+    In ctr (m_contracts s1) ->
+    ~ In (Executed ctr_id) (m_events s1) ->
+    In (Executed ctr_id) (m_events s2) ->
+    O <> 0 ->
+    (exists time tr,
+      In tr (m_ledger s2) /\
+      tr_ctr_id tr = ctr_id /\
+      tr_from tr = I /\
+      tr_to tr = O /\
+      tr_amount tr = sc * 11 /\
+      tr_timestamp tr = time) \/
+    exists ctr,
+      In ctr (m_contracts s2) /\
+      ctr_primitive ctr = (At (now + period) (Scale 11 (One USD))) /\
+      ctr_issuer ctr = I /\
+      ctr_owner ctr = O /\
+      ctr_scale ctr = sc.
+Proof.
+  intros.
+  induction H.
+  - subst. contradiction.
+  - assert (H' := H). assert (H'' := H).
+    apply steps_preserves_consistent_state in H'; auto.
+    apply steps_effect_over_contract with (ctr := ctr) in H; trivial.
+    destruct H as [H|[H|H]]; trivial.
+    + eapply zcb_step_I_to_O_new_ctr; eauto.
+      destruct H' as [_ [_ [_ [H' _]]]].
+      apply H' in H.
+      destruct H as [H _].
+      subst ctr. simpl in H. trivial.
+    + subst ctr. simpl in H.
+      apply IHsteps in H.
+      destruct H as [[t [tr [H A]]] | [ctr [H [A1 [A2 [A3 A4]]]]]].
+      * left. exists t, tr.
+        split; trivial.
+        eapply step_does_not_remove_transactions; eauto.
+      * clear H2 H3 H4. clear IHsteps.
+        apply step_effect_over_contract with (ctr := ctr) in H6.
+        destruct H6 as [H6 | [H6 | H6]].
+        ** right. exists ctr. repeat split; trivial.
+        ** left. 
+        induction H6; subst s2; simpl in *.
+        ** 
+
+        right. exists ctr.
+        split; trivial.
+
+
+
+
+  - simpl in *. destruct H4 as [H4 | H4]; try inversion H4.
+    contradiction.
+  - simpl in *. unfold exec_ctr_in_state_with_owner in H11.
+    unfold can_join in H6.
+    destruct H6 as [H6 | H6]; intros.
+    case_eq (ctr_eq_dec ctr ctr0); intros; try contradiction.
+    subst ctr0 ctr.
+    apply zcb_execute_I_to_O_new_ctr in H11.
+    simpl in *.
+    destruct H11 as
+        [[tr (A1 & A2 & A3 & A4 & A5 & A6)] |
+         [ctr (A1 & A2 & A3 & A4 & A5 )]].
+    + subst. left. exists (m_global_time s1), tr.
+      repeat split; trivial.
+    + subst. right. exists ctr.
+      repeat split; trivial.
+      apply in_app_iff. right. trivial.
+    + case_eq (ctr_eq_dec ctr ctr0); intros; try contradiction.
+      subst ctr0 ctr.
+      simpl in H6. subst O. contradiction.
+  - case_eq (ctr_eq_dec ctr ctr0); intros; try contradiction.
+    subst ctr0 ctr. unfold zcb_desc in *. simpl in *. inversion H8.
+  - case_eq (ctr_eq_dec ctr ctr0); intros; try contradiction.
+    subst ctr0 ctr. unfold zcb_desc in *. simpl in *. inversion H8.
+  - simpl in *. destruct H4 as [H4 | H4]. inversion H4. contradiction.
+  - simpl in *. contradiction.
+Qed.
+
+Lemma zcb_steps_I_to_O :
+  forall s1 s2 ctr_id dsc_id now period I O sc ctr,
+    steps s1 s2 ->
+    consistent_state s1 ->
+    ctr = finctr ctr_id dsc_id (zcb_desc now period) I O O sc ->
+    In ctr (m_contracts s1) ->
+    ~ In (Executed ctr_id) (m_events s1) ->
+    In (Executed ctr_id) (m_events s2) ->
+    O <> 0 ->
+    (exists time tr,
+      In tr (m_ledger s2) /\
+      tr_ctr_id tr = ctr_id /\
+      tr_from tr = I /\
+      tr_to tr = O /\
+      tr_amount tr = sc * 11 /\
+      tr_timestamp tr = time) \/
+    exists ctr,
+      In ctr (m_contracts s2) /\
+      ctr_primitive ctr = (At (now + period) (Scale 11 (One USD))) /\
+      ctr_issuer ctr = I /\
+      ctr_owner ctr = O /\
+      ctr_scale ctr = sc.
+Proof.
+  intros.
+  induction H.
+  - subst. contradiction.
+  - apply zcb_execute_I_to_O_new_ctr in H6.
+    assert (H' := H). assert (H'' := H).
+    apply steps_preserves_consistent_state in H'; auto.
+    apply steps_effect_over_contract with (ctr := ctr) in H; trivial.
+    destruct H as [H|[H|H]]; trivial.
+    + eapply zcb_execute_I_to_O_new_ctr in H9.
+
+
+zcb_execute_I_to_O_new_ctr
+
+
+Lemma zcb_steps_I_to_O :
+  forall s1 s2 ctr_id dsc_id now period I O sc ctr,
+    steps s1 s2 ->
+    consistent_state s1 ->
+    ctr = finctr ctr_id dsc_id (zcb_desc now period) I O O sc ->
+    In ctr (m_contracts s1) ->
+    ~ In (Executed ctr_id) (m_events s1) ->
+    In (Executed ctr_id) (m_events s2) ->
+    O <> 0 ->
+    m_global_time s1 = now ->
+    m_global_time  s2 = (now + period) ->
+    Δ <= now + period ->
+    exists time tr,
+      In tr (m_ledger s2) /\
+      tr_ctr_id tr = ctr_id /\
+      tr_from tr = I /\
+      tr_to tr = O /\
+      tr_amount tr = sc * 11 /\
+      tr_timestamp tr = time.
+Proof.
+  intros.
+  induction H.
+  - subst. contradiction.
+  - assert (H' := H). assert (H'' := H).
+    apply steps_preserves_consistent_state in H'; auto.
+    apply steps_effect_over_contract with (ctr := ctr) in H; trivial.
+    destruct H as [H|[H|H]]; trivial.
+    + eapply zcb_step_I_to_O; eauto.
+      * destruct H' as [_ [_ [_ [H' _]]]].
+        apply H' in H.
+        destruct H as [H _]. subst ctr. simpl in H. trivial.
+      * eapply no_tick_if_event_generated'; eauto.
+        exists (Executed ctr_id0).
+        split; auto.
+        destruct H' as [_ [_ [_ [H' _]]]].
+        apply H' in H.
+        destruct H as [H _]. subst ctr. simpl in H. trivial.
+    + subst ctr. simpl in H.
+      eapply IHsteps in H. clear IHsteps.
+      * destruct H as [time [tr [H HT]]].
+        exists time, tr.
+        split; trivial.
+        eapply steps_does_not_remove_transactions; eauto.
+        eapply tran; eauto. eapply refl. trivial.
+      * apply time_passes_one_step_at_a_time' with (n := now + period - 1)in H9.
+        clear H2 IHsteps.
+        destruct H9 as [H9 | H9].
+        ** admit.
+        ** admit.
+        ** 
+        
+    + subst ctr. simpl in H.
+      assert (TH: In (Deleted ctr_id0) (m_events s2)).
+      eapply step_does_not_remove_events; eauto.
+      apply step_preserves_consistent_state with (s' := s2)in H'; auto.
+      destruct H' as [_ [_ [_ [_ H']]]].
+      unfold not in H'.
+      exfalso.
+      eapply H'; eauto.
+Admitted.
+
+
+
 
 
 Definition zcb
